src/mqtt-packet-parser/src/connect.fst
@@ -1,11 +1,17 @@
 module Connect
 
+module U8 = FStar.UInt8
+module U32 = FStar.UInt32
+module B = LowStar.Buffer
+
+open C.String
+open LowStar.BufferOps
+open FStar.HyperStack.ST
+open FStar.Int.Cast
+
 open Const
 open Common
 
-open C.String
-
-module U8 = FStar.UInt8
 
 val assemble_connect_struct: s: struct_connect_parts
   -> Pure struct_fixed_header
@@ -79,3 +85,183 @@ let assemble_connect_struct s =
       message = define_no_error;
     };
   }
+
+val connect_packet_parser: packet_data: (B.buffer U8.t) 
+  -> packet_size: type_packet_size 
+  -> next_start_index:U32.t
+  -> Stack (connect_packet_seed: struct_connect_packet_seed)
+    (requires fun h0 -> B.live h0 packet_data)
+    (ensures fun h0 r h1 -> true)
+let connect_packet_parser packet_data packet_size next_start_index =
+  push_frame ();
+  let ptr_is_break: B.buffer bool = B.alloca false 1ul in
+  let ptr_protocol_name_error_status: B.buffer U8.t = B.alloca 0uy 1ul in
+  let ptr_protocol_version_error_status: B.buffer U8.t = B.alloca 0uy 1ul in
+  let ptr_connect_flag: B.buffer U8.t = B.alloca 0uy 1ul in
+  let ptr_keep_alive: B.buffer U8.t = B.alloca 0uy 2ul in
+  let ptr_connect_topic_length: B.buffer U32.t = B.alloca 0ul 1ul in
+  let ptr_connect_property_id: B.buffer U8.t = B.alloca 0uy 1ul in
+  let inv h (i: nat) =
+    B.live h packet_data /\
+    B.live h ptr_is_break /\
+    B.live h ptr_protocol_name_error_status /\
+    B.live h ptr_protocol_version_error_status /\
+    B.live h ptr_connect_flag /\
+    B.live h ptr_keep_alive /\
+    B.live h ptr_connect_topic_length /\
+    B.live h ptr_connect_property_id
+    in
+  let body (i: U32.t{ 2 <= U32.v i && U32.v i < U32.v packet_size  }): Stack unit
+    (requires (fun h -> inv h (U32.v i)))
+    (ensures (fun _ _ _ -> true))
+  =
+    let one_byte : U8.t = packet_data.(i) in
+    let is_break: bool = ptr_is_break.(0ul) in
+    if (is_break) then
+      ()
+    else
+      (
+        let variable_header_index = U32.sub i next_start_index in
+        if (U32.lte variable_header_index 5ul) then
+          (
+            if (
+              (U32.eq variable_header_index 0ul && not (U8.eq one_byte 0x00uy)) ||
+              (U32.eq variable_header_index 1ul && not (U8.eq one_byte 0x04uy)) ||
+              (U32.eq variable_header_index 2ul && not (U8.eq one_byte 0x4Duy)) ||
+              (U32.eq variable_header_index 3ul && not (U8.eq one_byte 0x51uy)) ||
+              (U32.eq variable_header_index 4ul && not (U8.eq one_byte 0x54uy)) ||
+              (U32.eq variable_header_index 5ul && not (U8.eq one_byte 0x54uy))
+              ) then
+              (
+                ptr_protocol_name_error_status.(0ul) <- 1uy;
+                ptr_is_break.(0ul) <- true
+              )
+          )
+          else if (U32.eq variable_header_index 6ul && not (U8.eq one_byte 0x05uy)) then
+            (
+              ptr_protocol_version_error_status.(0ul) <- 1uy;
+              ptr_is_break.(0ul) <- true
+            )
+          else if (U32.eq variable_header_index 7ul) then
+            (
+              ptr_connect_flag.(0ul) <- one_byte
+            )
+          else if (U32.eq variable_header_index 8ul) then
+            (
+              ptr_keep_alive.(0ul) <- one_byte
+            )
+          else if (U32.eq variable_header_index 9ul) then
+            (
+              if (U8.lte one_byte 0x7Fuy) then
+                (
+                  ptr_keep_alive.(1ul) <- one_byte
+                )
+              // else 
+              //   (
+              //     // TODO: keep aliveが127以上の場合は未実装.
+              //   )
+            )
+          else if (U32.eq variable_header_index 10ul) then
+            (
+              // TODO: topic length が一桁かつ, keep aliveが127以下の場合
+              ptr_connect_topic_length.(0ul) <- uint8_to_uint32 one_byte
+            )
+          else if (U32.eq variable_header_index 11ul) then
+            (
+              // TODO: topic length が一桁かつ, keep aliveが127以下の場合
+              ptr_connect_property_id.(0ul) <- one_byte
+            )
+          // else
+          //   (
+          //     print_string "x: ";
+          //     print_u8 one_byte;
+          //     print_string ", index: ";
+          //     print_u32 variable_header_index;
+          //     print_string "\n"
+          //   )
+      )
+  in
+  C.Loops.for next_start_index packet_size inv body;
+
+  let protocol_name_error_status: U8.t = ptr_protocol_name_error_status.(0ul) in
+  let protocol_version_error_status: U8.t = ptr_protocol_version_error_status.(0ul) in
+  let connect_flag: U8.t = ptr_connect_flag.(0ul) in
+  let keep_alive_msb_u8: U8.t = ptr_keep_alive.(0ul) in
+  let keep_alive_lsb_u8: U8.t = ptr_keep_alive.(1ul) in
+  let connect_topic_length: U32.t = ptr_connect_topic_length.(0ul) in
+  let connect_property_id: U8.t = ptr_connect_property_id.(0ul) in
+  pop_frame ();
+
+  let connect_packet_seed: struct_connect_packet_seed = {
+    connect_seed_protocol_name_error_status = protocol_name_error_status;
+    connect_seed_protocol_version_error_status = protocol_version_error_status;
+    connect_seed_connect_flag = connect_flag;
+    connect_seed_keep_alive_msb_u8 = keep_alive_msb_u8;
+    connect_seed_keep_alive_lsb_u8 = keep_alive_lsb_u8;
+    connect_seed_connect_topic_length = connect_topic_length;
+    connect_seed_connect_property_id = connect_property_id;
+  } in connect_packet_seed
+
+val connect_packet_parse_result: (share_common_data: struct_share_common_data)
+  -> Stack (r: struct_fixed_header)
+    (requires fun h0 -> B.live h0 share_common_data.common_packet_data)
+    (ensures fun h0 r h1 -> true)
+let connect_packet_parse_result share_common_data =
+  let connect_packet_seed: struct_connect_packet_seed = 
+  connect_packet_parser share_common_data.common_packet_data share_common_data.common_packet_size  share_common_data.common_next_start_index in
+  let connect_constant: struct_fixed_header_constant =
+    get_struct_fixed_header_constant_except_publish share_common_data.common_message_type in
+  let connect_flag: U8.t = connect_packet_seed.connect_seed_connect_flag in
+  let user_name_flag: U8.t = slice_byte connect_flag 0uy 1uy in
+  let password_flag: U8.t = slice_byte connect_flag 1uy 2uy in
+  let will_retain_flag: U8.t = slice_byte connect_flag 2uy 3uy in
+  let will_qos_flag: U8.t = slice_byte connect_flag 3uy 5uy in
+  let will_flag: U8.t = slice_byte connect_flag 5uy 6uy in
+  let clean_start_flag: U8.t = slice_byte connect_flag 6uy 7uy in
+  let resreved_flag: U8.t = slice_byte connect_flag 7uy 8uy in
+  let connect_property_id: U8.t = connect_packet_seed.connect_seed_connect_property_id in
+  let keep_alive_msb_u32: U32.t = 
+    uint8_to_uint32 connect_packet_seed.connect_seed_keep_alive_msb_u8  in
+  let keep_alive_lsb_u32: U32.t = 
+    uint8_to_uint32 connect_packet_seed.connect_seed_keep_alive_lsb_u8 in 
+  let keep_alive: U32.t = 
+    U32.logor (U32.shift_left keep_alive_msb_u32 8ul)keep_alive_lsb_u32 in
+
+  let have_error: bool =
+    (connect_packet_seed.connect_seed_protocol_name_error_status = 1uy) ||
+    (connect_packet_seed.connect_seed_protocol_version_error_status = 1uy) ||
+    (not (U8.eq resreved_flag 0uy) ) in
+  if (have_error) then
+    (
+      let error_struct: struct_error_struct =
+        (
+          if (connect_packet_seed.connect_seed_protocol_name_error_status = 1uy) then
+            {
+              code = define_error_protocol_name_invalid_code;
+              message = define_error_protocol_name_invalid;
+            }
+          else if (connect_packet_seed.connect_seed_protocol_version_error_status = 1uy) then
+            {
+              code = define_error_protocol_version_invalid_code;
+              message = define_error_protocol_version_invalid;
+            }
+          else // if (not (U8.eq resreved_flag 0uy) ) then
+            {
+              code = define_error_connect_flag_invalid_code;
+              message = define_error_connect_flag_invalid;
+            }
+        ) in error_struct_fixed_header error_struct
+    )
+  else
+    (
+      let ed_fixed_header_parts:
+        struct_connect_parts = {
+          connect_remaining_length = share_common_data.common_remaining_length;
+          connect_connect_constant = connect_constant;
+          connect_connect_flag = connect_flag;
+          connect_keep_alive = keep_alive;
+          connect_connect_topic_length = connect_packet_seed.connect_seed_connect_topic_length;
+          connect_connect_property_id = connect_packet_seed.connect_seed_connect_property_id;
+      } in
+      assemble_connect_struct ed_fixed_header_parts            
+    )
