src/mqtt-packet-parser/src/publish.fst
@@ -1,11 +1,17 @@
 module Publish
 
 module U8 = FStar.UInt8
+module U32 = FStar.UInt32
+module B = LowStar.Buffer
 
 open C.String
+open LowStar.BufferOps
+open FStar.HyperStack.ST
+open FStar.Int.Cast
 
 open Const
 open Common
+open FFI
 
 val get_dup_flag: fixed_header_first_one_byte: U8.t -> type_dup_flags_restrict
 let get_dup_flag fixed_header_first_one_byte =
@@ -101,3 +107,251 @@ let assemble_publish_struct s =
             message = define_no_error;
           };
         }
+
+val publish_packet_parser: packet_data: (B.buffer U8.t) 
+  -> packet_size: type_packet_size 
+  -> next_start_index:U32.t
+  -> Stack (publish_packet_seed: struct_publish_packet_seed)
+    (requires fun h0 -> B.live h0 packet_data)
+    (ensures fun h0 r h1 -> true)
+let publish_packet_parser packet_data packet_size next_start_index =
+  push_frame();
+  let ptr_is_break: B.buffer bool = B.alloca false 1ul in
+  let ptr_for_topic_length: B.buffer U8.t = B.alloca 0uy 1ul in
+  let ptr_topic_length: B.buffer type_topic_length_restrict = B.alloca max_u32 1ul in
+  let ptr_topic_name_u8: B.buffer U8.t = B.alloca 0uy 65536ul in
+  let ptr_topic_name: B.buffer type_topic_name_restrict = B.alloca !$"" 1ul in
+  let ptr_topic_name_error_status: B.buffer U8.t = B.alloca 0uy 1ul in
+  let ptr_property_length: B.buffer type_property_length = B.alloca 0ul 1ul in
+  let ptr_is_searching_property_length: B.buffer bool = B.alloca true 1ul in
+  let ptr_payload: B.buffer type_payload_restrict = B.alloca !$"" 1ul in
+  let ptr_payload_error_status: B.buffer U8.t = B.alloca 0uy 1ul in
+
+  let inv h (i: nat) =
+    B.live h packet_data /\
+    B.live h ptr_is_break /\
+    B.live h ptr_for_topic_length /\
+    B.live h ptr_topic_length /\
+    B.live h ptr_topic_name_u8 /\
+    B.live h ptr_topic_name /\
+    B.live h ptr_topic_name_error_status /\
+    B.live h ptr_property_length /\
+    B.live h ptr_is_searching_property_length /\
+    B.live h ptr_payload /\
+    B.live h ptr_payload_error_status
+    in
+  let body (i: U32.t{ 2 <= U32.v i && U32.v i < U32.v packet_size  }): Stack unit
+    (requires (fun h -> inv h (U32.v i)))
+    (ensures (fun _ _ _ -> true))
+  =
+    let one_byte : U8.t = packet_data.(i) in
+    let is_break: bool = ptr_is_break.(0ul) in
+    if (is_break) then
+      ()
+    else
+      (
+        let variable_header_index = U32.sub i next_start_index in
+        let topic_length: type_topic_length_restrict = ptr_topic_length.(0ul) in
+        if (variable_header_index = 0ul) then
+          ptr_for_topic_length.(0ul) <- one_byte
+        else if (variable_header_index = 1ul) then
+          (
+            let msb_u8: U8.t = ptr_for_topic_length.(0ul) in
+            let lsb_u8: U8.t = one_byte in
+            let msb_u32: U32.t = uint8_to_uint32 msb_u8  in
+            let lsb_u32: U32.t = uint8_to_uint32 lsb_u8 in
+            let _topic_length: U32.t =
+              U32.logor (U32.shift_left msb_u32 8ul) lsb_u32 in
+            if (U32.gt _topic_length 65535ul) then
+              (
+                ptr_topic_length.(0ul) <- max_u32;
+                ptr_is_break.(0ul) <- true
+              )
+            else
+              (
+                ptr_topic_length.(0ul) <- _topic_length
+              )
+          )
+        else if (U32.gte variable_header_index 2ul) then
+          (
+            let is_searching_property_length: bool =
+              ptr_is_searching_property_length.(0ul) in
+            if (topic_length = max_u32) then
+              (
+                ptr_topic_length.(0ul) <- max_u32;
+                ptr_is_break.(0ul) <- true
+              )
+            else
+              (
+              if (U32.lte variable_header_index (U32.(topic_length +^ 1ul))) then
+                (
+                  if (U8.eq one_byte 0x00uy || U8.eq one_byte 0x23uy || U8.eq one_byte 0x2buy) then
+                    (
+                      ptr_topic_name_error_status.(0ul) <- 2uy;
+                      ptr_is_break.(0ul) <- true
+                    )
+                  else
+                    (
+                      ptr_topic_name_u8.(U32.sub variable_header_index 2ul) <- one_byte;
+                      // 0xEF 0xBB 0xBF は 0xFE 0xFF 置換
+                      // ptr_topic_name_order_mark_check.(0ul) <- 0uy;
+                      if (variable_header_index = (U32.(topic_length +^ 1ul))) then
+                        (
+                          let topic_name: type_topic_name_restrict =
+                            (
+                              if (ptr_topic_name_u8.(65535ul) = 0uy) then
+                                let replace_bom = replace_utf8_encoded ptr_topic_name_u8 65536ul in
+                                topic_name_uint8_to_c_string replace_bom
+                              else
+                                (
+                                  ptr_topic_name_error_status.(0ul) <- 1uy;
+                                  !$""
+                                )
+                            ) in ptr_topic_name.(0ul) <- topic_name
+                        )
+                      )
+                )
+              else if (U32.gt variable_header_index (U32.(topic_length +^ 1ul))
+                && U32.lte variable_header_index (U32.(topic_length +^ 5ul))
+                && is_searching_property_length
+                ) then
+                (
+
+                  if (one_byte = 0uy) then
+                    (
+                      ptr_property_length.(0ul) <- uint8_to_uint32 one_byte;
+                      ptr_is_searching_property_length.(0ul) <- false
+                    )
+                    // else (
+                    //   // TODO: 3.3.2.3 PUBLISH Properties 
+                    //   // https://docs.oasis-open.org/mqtt/mqtt/v5.0/os/mqtt-v5.0-os.html#_Toc3901109
+                    //   // print_not_implemented "PUBLISH Properties Parsing"
+                    // )
+                )
+              else if (not is_searching_property_length) then
+                (
+                  let payload_offset: type_payload_offset = i in
+                  let ptr_payload_u8: B.buffer U8.t = B.offset packet_data payload_offset in
+                  let payload: type_payload_restrict =
+                    (
+                      let last_payload_index: U32.t =
+                        U32.(packet_size -^ payload_offset) in
+                      let last_payload_element: U8.t = ptr_payload_u8.(last_payload_index) in
+                        if (last_payload_element <> 0uy) then
+                          (
+                            ptr_payload_error_status.(0ul) <- 1uy;
+                            !$""
+                          )
+                        else
+                          payload_uint8_to_c_string ptr_payload_u8 min_packet_size max_packet_size packet_size
+                    ) in
+                  ptr_payload.(0ul) <- payload;
+                  ptr_is_break.(0ul) <- true
+                )
+              else
+                (
+                  ()
+                )
+              )
+          )
+        else
+          (
+            ()
+          )
+      )
+  in
+  C.Loops.for next_start_index packet_size inv body;
+  pop_frame ();
+
+  let topic_length: type_topic_length_restrict = ptr_topic_length.(0ul) in
+  let topic_name: type_topic_name_restrict = ptr_topic_name.(0ul) in
+  let topic_name_error_status: U8.t = ptr_topic_name_error_status.(0ul) in
+  let is_searching_property_length: bool = ptr_is_searching_property_length.(0ul) in
+  let property_length: type_property_length = ptr_property_length.(0ul) in
+  let payload: type_payload_restrict = ptr_payload.(0ul) in
+  let payload_error_status: U8.t = ptr_payload_error_status.(0ul) in
+
+  let publish_packet_seed: struct_publish_packet_seed = {
+    publish_seed_topic_length = topic_length;
+    publish_seed_topic_name = topic_name;
+    publish_seed_topic_name_error_status = topic_name_error_status;
+    publish_seed_is_searching_property_length = is_searching_property_length;
+    publish_seed_property_length = property_length;
+    publish_seed_payload = payload;
+    publish_seed_payload_error_status = payload_error_status;
+  } in publish_packet_seed
+
+val publish_packet_parse_result: (share_common_data: struct_share_common_data)
+  -> Stack (r: struct_fixed_header)
+    (requires fun h0 -> B.live h0 share_common_data.common_packet_data)
+    (ensures fun h0 r h1 -> true)
+let publish_packet_parse_result share_common_data =
+  let publish_packet_seed: struct_publish_packet_seed = 
+    publish_packet_parser share_common_data.common_packet_data share_common_data.common_packet_size share_common_data.common_next_start_index in
+  let first_one_byte: U8.t = share_common_data.common_first_one_byte in
+  let dup_flag: type_dup_flags_restrict = get_dup_flag first_one_byte in
+  let qos_flag: type_qos_flags_restrict = get_qos_flag first_one_byte in
+  let retain_flag: type_retain_flags_restrict = get_retain_flag first_one_byte in
+  let have_error: bool =
+    (U8.eq dup_flag max_u8) ||
+    (U8.eq qos_flag max_u8) ||
+    (U8.eq retain_flag max_u8) ||
+    (U32.eq publish_packet_seed.publish_seed_topic_length max_u32) ||
+    (U8.eq publish_packet_seed.publish_seed_topic_name_error_status 1uy) ||
+    (U8.eq publish_packet_seed.publish_seed_topic_name_error_status 2uy) ||
+    (publish_packet_seed.publish_seed_is_searching_property_length) ||
+    (U8.gt publish_packet_seed.publish_seed_payload_error_status 0uy) in
+  if (have_error) then
+    (
+      let error_struct: struct_error_struct =
+        (
+          if (U8.eq dup_flag max_u8) then
+            {
+              code = define_error_dup_flag_invalid_code;
+              message = define_error_dup_flag_invalid;
+            }
+          else if (U8.eq qos_flag max_u8) then
+            {
+              code = define_error_qos_flag_invalid_code;
+              message = define_error_qos_flag_invalid;
+            }
+          else if (U8.eq retain_flag max_u8) then
+            {
+              code = define_error_retain_flag_invalid_code;
+              message = define_error_retain_flag_invalid;
+            }
+          else if (U32.eq publish_packet_seed.publish_seed_topic_length max_u32) then
+            {
+              code = define_error_topic_length_invalid_code;
+              message = define_error_topic_length_invalid;
+            }
+          else if (U8.eq publish_packet_seed.publish_seed_topic_name_error_status 1uy) then
+            {
+              code = define_error_topic_name_dont_zero_terminated_code;
+              message = define_error_topic_name_dont_zero_terminated;
+            }
+          else if (U8.eq publish_packet_seed.publish_seed_topic_name_error_status 2uy) then
+            {
+              code = define_error_topic_name_have_inavlid_character_code;
+              message = define_error_topic_name_have_inavlid_character;
+            }
+          else // if (is_searching_property_length) then
+            {
+              code = define_error_property_length_invalid_code;
+              message = define_error_property_length_invalid;
+            }
+        ) in error_struct_fixed_header error_struct
+    )
+  else
+    (
+      let ed_fixed_header_parts:
+        struct_publish_parts = {
+          publish_fixed_header_first_one_byte = first_one_byte;
+          publish_remaining_length = share_common_data.common_remaining_length;
+          publish_topic_length = publish_packet_seed.publish_seed_topic_length;
+          publish_topic_name = publish_packet_seed.publish_seed_topic_name;
+          publish_property_length = publish_packet_seed.publish_seed_property_length;
+          publish_payload = publish_packet_seed.publish_seed_payload;
+      } in
+      assemble_publish_struct ed_fixed_header_parts
+    )
